Struct/Struct.lean
@@ -1,11 +1,9 @@
 import Lean
 
--- import Struct.Helpers
 import Struct.CustomTactics
 
 open 
   Lean 
-  Lean.Expr
   Lean.Meta 
   Lean.Elab 
   Lean.Elab.Tactic
@@ -13,20 +11,16 @@ open
   Lean.Parser 
   Lean.Parser.Tactic
 
--- TMP for debugging
-set_option pp.rawOnError true
-
 /-
-  # Description of this file ..
+  # Stuct - Core of the `structured` tactic
+
+  
 
 -/
 
--- ## State to tactic(Seq) builders
-def mkShow (newGoalTerm : Term) (tacSeq : TSyntax ``tacticSeq) : TermElabM (TSyntax `tactic) := do
-  `(tactic|show $newGoalTerm by $tacSeq)
- 
+-- ## xx
 def mkSuffices (newGoalTerm : Term) (tacSeq : TSyntax ``tacticSeq) : TermElabM (TSyntax `tactic) := do
-  `(tactic|suffices $newGoalTerm by $tacSeq)
+  `(tactic|s_suffices $newGoalTerm:term by $tacSeq)
 
 def mkHave (decl : LocalDecl) (tacSeq : TSyntax ``tacticSeq) : TermElabM (TSyntax `tactic) := do
   let declType ← delab (← instantiateMVars decl.type)
@@ -34,28 +28,39 @@ def mkHave (decl : LocalDecl) (tacSeq : TSyntax ``tacticSeq) : TermElabM (TSynta
   | true => 
     let id := mkIdent decl.userName
     `(tactic|have $id : $declType := by $tacSeq)
-  | false => 
-    `(tactic|have : $declType := by $tacSeq)
+  | false =>
+    let nameBase := if ← isProp decl.type then "h" else "a"
+    let autoName := mkIdent $ (← getLCtx).getUnusedName (.str .anonymous nameBase)
+    `(tactic|have $autoName : $declType := by $tacSeq)
 
-def mkFix (decls : Array LocalDecl) (goal : Term) : TermElabM (TSyntax `tactic) := do
-  let binders ← decls.mapM (fun decl => declToBinder decl)
-  `(tactic|fix $[$binders]* ⊢ $goal)
 
-def mkNote (decls : Array LocalDecl := #[]) (optGoal : Option Term := none) (optTacSeq : Option (TSyntax ``tacticSeq)) : TermElabM (TSyntax `tactic) := do
+def mkSuggestion (decls : Array LocalDecl := #[]) (optGoal : Option Term := none) (optTacSeq : Option (TSyntax ``tacticSeq)) : TermElabM (TSyntax `tactic) := do
   let binders ← decls.mapM (fun decl => declToBinder decl)  
   match optGoal with
   | some goal => 
     match optTacSeq with
-    | some tacSeq => `(tactic|note $[$binders]* ⊢ $goal by $tacSeq)
-    | none => `(tactic|show $[$binders]* ⊢ $goal)
-  | none => 
-    match optTacSeq with
-    | some tacSeq => `(tactic|note $[$binders]* by $tacSeq)
+    | some tacSeq => 
+      if binders.size == 0 then
+        `(tactic|s_suffices $goal:term by $tacSeq)    
+      else
+        `(tactic|s_suffices $[$binders]* ⊢ $goal by $tacSeq)
     | none => 
       if binders.size == 0 then
-        throwError "Nothing to note, TODO"
+        `(tactic|show $goal)
       else
-        `(tactic|note $[$binders]*)
+        `(tactic|s_show $[$binders]* ⊢ $goal)
+  | none => 
+    match optTacSeq with
+    | some tacSeq => 
+      if binders.size == 0 then
+        throwError "No change of state detected, unreachable state, this should be caught by goal comparison match"
+      else
+        `(tactic|s_have $[$binders]* by $tacSeq)
+    | none => 
+      if binders.size == 0 then
+        throwError "No change of state detected, unreachable state, this should be caught by goal comparison match"
+      else
+        `(tactic|s_have $[$binders]*)
 
 
 -- ## Segment description
@@ -85,10 +90,10 @@ def goalsToStateDiff (oldGoal : MVarId) (newGoal : MVarId) : TacticM StateDiff :
   let mut removedDecls := #[]
 
   for newDecl in newLCtx do
-    if !newDecl.isAuxDecl then -- todo isImplementationDetail
+    if !newDecl.isImplementationDetail then
       let mut foundMatch : Bool := false
       for oldDecl in oldLCtx do
-        if !oldDecl.isAuxDecl then
+        if !oldDecl.isImplementationDetail then
           if newDecl.userName == oldDecl.userName then
             foundMatch := true
             if !(newDecl.type.consumeMData == oldDecl.type.consumeMData) then
@@ -108,10 +113,29 @@ def goalsToStateDiff (oldGoal : MVarId) (newGoal : MVarId) : TacticM StateDiff :
 
   return StateDiff.mk newlyChangedGoal newDecls changedDecls removedDecls
 
+def mkNameFromTerm (type : Term) : TacticM (TSyntax `ident) := do
+  let elaboratedTerm ← elabTerm type none
+  let nameBase := if (← isProp elaboratedTerm) then "h" else "a"
+  let ident := mkIdent $ (← getLCtx).getUnusedName (.str .anonymous nameBase)
+  return ident
+
+def mkTypeFromTac (rhs : TSyntax `tactic) : TacticM (TSyntax `term) := 
+  withoutModifyingState do
+    let oldGoal ← getMainGoal
+    evalTactic rhs
+    let newGoal ← getMainGoal
+    let s ← goalsToStateDiff oldGoal newGoal
+    match (s.newDecls, s.changedDecls) with
+    | (#[decl], #[]) => 
+      return ← delab (← instantiateMVars decl.type)
+    | (#[], #[decl]) => 
+      return ← delab (← instantiateMVars decl.type)
+    | _ => throwError "Not a single hypothesis change detected"
+
 def mapMVarToNote (oldGoal : MVarId) (newGoal : MVarId) : TacticM (TSyntax `tactic) := do
   newGoal.withContext do
     let s ← goalsToStateDiff oldGoal newGoal
-    mkNote (s.changedDecls ++ s.newDecls) s.newlyChangedGoal none
+    mkSuggestion (s.changedDecls ++ s.newDecls) s.newlyChangedGoal none
 
 def getNotesFromTac (oldGoal : MVarId) (tac : TSyntax `tactic) : TacticM (List (TSyntax `tactic)) := do
   oldGoal.withContext do
@@ -131,7 +155,7 @@ def getTacs (ts : TSyntax ``tacticSeq) : TermElabM (Array (TSyntax `tactic)) :=
   match ts with
   | `(tacticSeq| { $[$tacs:tactic]* }) => return tacs
   | `(tacticSeq| $[$tacs:tactic]*) => return tacs
-  | _ => throwError "unknown syntax"
+  | _ => throwUnsupportedSyntax
 
 def replaceHoleWithNoteInductionAlt (old : TSyntax ``inductionAlt) (note : TSyntax `tactic) : TermElabM (TSyntax ``inductionAlt) := do
   match old with
@@ -139,7 +163,7 @@ def replaceHoleWithNoteInductionAlt (old : TSyntax ``inductionAlt) (note : TSynt
       `(inductionAlt| | $lhs $[$ids]* => 
         $note:tactic)
   | _ => 
-    throwError "Shouldnt reach"
+    throwUnsupportedSyntax
 
 def replaceHoleWithNoteCaseTactic (old : TSyntax `tactic) (note : TSyntax `tactic) : TermElabM (TSyntax `tactic) := do
   match old with
@@ -147,27 +171,55 @@ def replaceHoleWithNoteCaseTactic (old : TSyntax `tactic) (note : TSyntax `tacti
       `(tactic|case $tag $[$ids]* => 
         $note:tactic)
   | _ => 
-    throwError "Shouldnt reach"
+    throwUnsupportedSyntax
 
+-- Function that turns a specific TSyntax to a more generic TSyntax
+def mapBinderIdentToTerm (id : TSyntax ([`ident, `Lean.Parser.Term.hole])): TacticM (TSyntax `term) := do 
+  match id with 
+  | `(term|$id) => `(term|$id)
 
 -- ## Structured branches
-def structuredIntros (tacSeq : TSyntax ``tacticSeq) (oldGoal : MVarId) : TacticM Unit := do
-  addTrace `xx m!"Testxx"
-  evalTactic tacSeq
-  match (← getUnsolvedGoals) with
-  | [] => throwError "Finishing with intros should be impossible"
-  | [newGoal] => 
-    let s ← goalsToStateDiff oldGoal newGoal
+def structuredIntros (target : Expr) (terms : TSyntaxArray `term) : TacticM Unit := do
+  forallBoundedTelescope target (some terms.size) fun fvarExprs _ => do 
+    let mut lctx ← getLCtx
+    let mut types := #[]
+    let mut binders := #[]
+    let localInsts <- getLocalInstances
+    for t in terms, fvarExpr in fvarExprs do
+      match fvarExpr with
+      | .fvar fvarId =>
+        let typeExpr := (← fvarId.getDecl).type
+        let type <- withLCtx lctx localInsts $ delab typeExpr
+        let baseAutoName := if ← isProp typeExpr then "h" else "a"
+        types := types.push type
 
-    match (s.newlyChangedGoal, s.newDecls, s.changedDecls, s.removedDecls) with
-    | ((some newGoalTerm), newDecls, changedDecls, #[]) => 
-      let suggestion ← mkFix (newDecls ++ changedDecls) newGoalTerm
-      addTrace `structured m!"Try this: {suggestion}"
-    | _ => throwError "Unexpected state: {StateDiff.toMessageData s}"
-  | _ => throwError "Unexpected state: Multiple goals after executing intro statement"
+        match t with
+        | `( _ ) =>
+          let autoName := lctx.getUnusedName (.str .anonymous baseAutoName)
+          lctx := lctx.setUserName fvarId autoName
+          binders := binders.push (← `(term| ($(mkIdent autoName) : $type)))
+          addTrace `xx m!"From underscore to ({autoName} : {type})"
+        | `( $id:ident ) =>
+          -- TODO verify id available
+          binders := binders.push (← `(term| ($id : $type)))
+          addTrace `xx m!"From only ident to ({id} : {type})"
+        | `( ( _ : $t:term) ) =>
+          let autoName := lctx.getUnusedName (.str .anonymous baseAutoName)
+          lctx := lctx.setUserName fvarId autoName
+          binders := binders.push (← `(term| ($(mkIdent autoName) : $t)))
+          addTrace `xx m!"From only type to ({autoName} : {t})"
+        | `( ($id:ident : $t:term) ) =>
+          -- TODO: verify id available
+          binders := binders.push (← `(term| ($id : $t)))
+          addTrace `xx m!"This is a binder with ident, already structured"
+        | _ =>
+          binders := binders.push (← `(term| ($t : $type)))
+          addTrace `xx m!"From dark magic to ({t} : {type})"
+      | _ => throwUnsupportedSyntax
+    let suggestion ← `(tactic|intro $[$binders]*)
+    addTrace `test m!"Try this: {suggestion}"
 
 -- TODO : Refactor out stuff
-
 def structuredCasesOrInduction (tacSeq : TSyntax ``tacticSeq) (oldGoal : MVarId) (target : TSyntax `term) (isInduction : Bool) : TacticM Unit :=
   oldGoal.withContext do
     let mut cases : Array (TSyntax ``inductionAlt) := #[]
@@ -176,7 +228,7 @@ def structuredCasesOrInduction (tacSeq : TSyntax ``tacticSeq) (oldGoal : MVarId)
 
     let targetExpr ← elabTerm target none
     let targetType ← inferType targetExpr
-    let fnExpr := getAppFn targetType
+    let fnExpr := targetType.getAppFn
     
     match fnExpr with
     | .const fnName _ =>
@@ -200,22 +252,21 @@ def structuredCasesOrInduction (tacSeq : TSyntax ``tacticSeq) (oldGoal : MVarId)
 
             for decl in decls do
               if decl.userName.hasMacroScopes then
-                let ctorName := (← getLCtx).getUnusedName (.str .anonymous "a")
+                let baseName := if ← isProp decl.type then "h" else "a"
+                let ctorName := (← getLCtx).getUnusedName (.str .anonymous baseName)
                 ctorArgs := ctorArgs.push (mkIdent ctorName)
 
-                if isInduction ∧ isAppOf decl.type fnName then
+                if isInduction ∧ decl.type.isAppOf fnName then
                   let indName := (← getLCtx).getUnusedName (.str ctorName "ih")
                   indArgs := indArgs.push (mkIdent indName)
               else
                 let ctorName := (← getLCtx).getUnusedName decl.userName
                 ctorArgs := ctorArgs.push (mkIdent ctorName)
 
-                if isInduction ∧ isAppOf decl.type fnName then
-                  -- Use previous human-readable userIdent and attempt to make that + "ih"
+                if isInduction ∧ decl.type.isAppOf fnName then
                   let indName := (← getLCtx).getUnusedName (.str ctorName "ih")
                   indArgs := indArgs.push (mkIdent indName)
             
-            -- TODO consider ?_ instead of skip
             let case ← `(inductionAlt| | $ctorIdent $[$ctorArgs]* $[$indArgs]* => ?_)
             cases := cases.push case
 
@@ -223,16 +274,13 @@ def structuredCasesOrInduction (tacSeq : TSyntax ``tacticSeq) (oldGoal : MVarId)
           
         | _ => addTrace `xx m!"Unexpected state 01"
       
-      -- Do stuff with cases, find out mvars inside
-      -- TODO if then else
-      match isInduction with
-      | true => 
+      if isInduction then
         let matchWithoutNotes ← `(tactic| induction $target:term with $[$cases]*)
         let notes ← getNotesFromTac oldGoal matchWithoutNotes
         let casesWithNotes ← cases.zip notes.toArray |>.mapM (fun (case, note) => do replaceHoleWithNoteInductionAlt case note)
         let matchWithNotes ← `(tactic| induction $target:term with $[$casesWithNotes]*)
         addTrace `test m!"Try this: {matchWithNotes}"
-      | false => 
+      else
         let matchWithoutNotes ← `(tactic| cases $target:term with $[$cases]*)
         let notes ← getNotesFromTac oldGoal matchWithoutNotes
         let casesWithNotes ← cases.zip notes.toArray |>.mapM (fun (case, note) => do replaceHoleWithNoteInductionAlt case note)
@@ -241,7 +289,7 @@ def structuredCasesOrInduction (tacSeq : TSyntax ``tacticSeq) (oldGoal : MVarId)
     | _ => addTrace `xx m!"Unexpected state 00"
 
 -- structuredCasesDefault: When multiple post-goals, but no match on cases or induction
-def structureCasesDefault (tacSeq : TSyntax ``tacticSeq) (oldGoal : MVarId) (newGoals : List MVarId) : TacticM Unit := do
+def structuredCasesDefault (tacSeq : TSyntax ``tacticSeq) (oldGoal : MVarId) (newGoals : List MVarId) : TacticM Unit := do
   let mut cases : Array (TSyntax `tactic) := #[]
 
   -- Construct a case for each new goal
@@ -253,7 +301,8 @@ def structureCasesDefault (tacSeq : TSyntax ``tacticSeq) (oldGoal : MVarId) (new
     let mut caseArgs : Array (TSyntax ``binderIdent) := #[]
     for decl in s.newDecls do
       if decl.userName.hasMacroScopes then
-        let caseArgName := (← newGoal.getDecl).lctx.getUnusedName (.str .anonymous "a") 
+        let baseName := if ← isProp decl.type then "h" else "a"
+        let caseArgName := (← newGoal.getDecl).lctx.getUnusedName (.str .anonymous baseName) 
         let caseArgIdent := mkIdent caseArgName
         caseArgs := caseArgs.push (← `(binderIdent|$caseArgIdent:ident))
 
@@ -268,8 +317,6 @@ def structureCasesDefault (tacSeq : TSyntax ``tacticSeq) (oldGoal : MVarId) (new
   let notes ← getNotesFromTacSeq oldGoal casesWithoutNotes
   let casesWithNotes ← cases.zip notes.toArray |>.mapM (fun (case, note) => do replaceHoleWithNoteCaseTactic case note)
 
-  addTrace `xx m!"Test: {casesWithoutNotes} {casesWithNotes}"
-
   -- Append all 
   let suggestion ← mkTacticSeqAppendTacs tacSeq casesWithNotes
   addTrace `structured m!"Try this: {suggestion}"
@@ -278,8 +325,7 @@ def structuredDefault (tacSeq : TSyntax ``tacticSeq) (oldGoal : MVarId) : Tactic
   evalTactic tacSeq
   match (← getUnsolvedGoals) with
   | [] => 
-    let suggestion ← mkShow (← delab (← oldGoal.getDecl).type) tacSeq
-    addTrace `structured m!"Try this: {suggestion}"
+    addTrace `structured m!"Goal finished, no need to add structure!"
   | [newGoal] => 
     let s ← goalsToStateDiff oldGoal newGoal
 
@@ -289,48 +335,110 @@ def structuredDefault (tacSeq : TSyntax ``tacticSeq) (oldGoal : MVarId) : Tactic
     | ((some newGoal), #[], #[], #[]) => 
       let suggestion ← mkSuffices newGoal tacSeq
       addTrace `structured m!"Try this: {suggestion}"
-    | (none, #[newDecl], #[], #[]) => -- TODO, can you both match on having nonzero newDecls, and name it so we can use it
+    | (none, #[newDecl], #[], #[]) =>
       let suggestion ← mkHave newDecl tacSeq
       addTrace `structured m!"Try this: {suggestion}"
     | (newlyChangedGoal, newDecls, changedDecls, #[]) =>
-      let suggestion ← mkNote (newDecls ++ changedDecls) newlyChangedGoal tacSeq
+      let suggestion ← mkSuggestion (newDecls ++ changedDecls) newlyChangedGoal tacSeq
       addTrace `structured m!"Try this: {suggestion}"
     | _ => 
       throwError "Unexpected state: Currently only occurs if any local declaration is lost after tactic evaluation.
                   Removed Declarations: {s.removedDecls.map (fun ldecl => ldecl.type)}"
 
   | newGoals => 
-    structureCasesDefault tacSeq oldGoal newGoals
-    pure ()
+    structuredCasesDefault tacSeq oldGoal newGoals
 
 -- ## Core structured elaboration
 def structuredCore (tacSeq : TSyntax ``tacticSeq) : TacticM Unit := do
   match (← getUnsolvedGoals) with
   | [] => 
-    logWarning m!"No goals to solve, kind of shouldn't reach this, since we can't execute your tactic anyways"
+    logWarning m!"No goals to solve, shouldn't reach this, since we can't execute your tactic anyways"
   | [goal] => 
     let tacs ← getTacs tacSeq
+    let goalType := (← goal.getDecl).type
     match tacs with
     | #[] => logWarning "No tactics in tacSeq"
-    -- TODO: Match on alternatives of existing structured tactics (from/by, etc)
     | #[t] =>
       match t with
-      -- Matching `suffices` Syntax
-      | `(tactic|suffices $_ by $_) 
-      | `(tactic|show $_ by $_) 
-      | `(tactic|have $[$id]? : $_ := by $_) 
-      | `(tactic|have $[$id]? : $_ := $_) 
+      -- Native Lean 4 tactics
+      | `(tactic|suffices $_) 
+      | `(tactic|show $_) 
       | `(tactic|clear $_)
+      | `(tactic|have $id:ident : $t:term := $rhs)
+      | `(tactic|let $id:ident : $t:term := $rhs)
+      -- Custom tactics
+      | `(tactic|s_suffices $[$bs]* ⊢ $_ by $_)
+      | `(tactic|s_suffices $_:term by $_)
+      | `(tactic|s_have $[$bs]* by $_)
+      | `(tactic|s_have $[$bs]*)
+      | `(tactic|s_show $[$bs]* ⊢ $_)
         => 
         addTrace `structured m!"This tactic is already structured"
         evalTactic tacSeq
-      -- TODO: Only match on intro $_, then unpack the content further in structuredIntros
-      | `(tactic|intro $[$ids:ident]*)
-      -- | `(tactic|intros $ids*)
+
+      | `(tactic|have $h:hole : $type:term := $rhs) -- hole-named typed
+        =>
+          let autoName ← mkNameFromTerm type
+          let suggestion ← `(tactic|have $autoName : $type := $rhs)
+          addTrace `structured m!"Try this: {suggestion}"
+      | tac@`(tactic|have $id:ident := $rhs) -- named untyped
+        =>
+          let autoType ← mkTypeFromTac tac
+          let suggestion ← `(tactic|have $id : $autoType := $rhs)
+          addTrace `structured m!"Try this: {suggestion}"
+      | tac@`(tactic|have $h:hole := $rhs) -- hole-named untyped
+      | tac@`(tactic|have := $rhs) -- unnamed untyped
+        =>
+          let autoType ← mkTypeFromTac tac
+          let autoName ← mkNameFromTerm autoType
+          let suggestion ← `(tactic|have $autoName : $autoType := $rhs)
+          addTrace `structured m!"Try this: {suggestion}"
+
+      | `(tactic|let $h:hole : $type:term := $rhs)  -- hole-named typed
         => 
-        let ids : Array (TSyntax `ident) := ids -- TODO mwe Zulip
-        addTrace `xx m!"{ids.map (fun x => repr x.raw)}"
-        structuredIntros tacSeq goal
+          let autoName ← mkNameFromTerm type
+          let suggestion ← `(tactic|let $autoName : $type := $rhs)
+          addTrace `structured m!"Try this: {suggestion}"
+      | tac@`(tactic|let $h:hole := $rhs) -- hole-named untyped    
+        => 
+          let autoType ← mkTypeFromTac tac
+          let autoName ← mkNameFromTerm autoType
+          let suggestion ← `(tactic|let $autoName : $autoType := $rhs)
+          addTrace `structured m!"Try this: {suggestion}"
+
+      | tac@`(tactic|intro $ts:term*) 
+        => 
+          evalTactic tac
+          withMainContext do
+            -- If intro is called anonymously, manually add the hole for easier function
+            if ts.size == 0 then do
+              let hole ← `( _ )
+              structuredIntros goalType #[hole]
+            else
+              structuredIntros goalType ts
+
+      | tac@`(tactic|intros $ids*)
+        => 
+          evalTactic tac
+          withMainContext do
+            if ids.size == 0 then do
+              -- The procedure to handle unbounded intros is to execute tactic
+              -- And compare goals, the amount of newDecls is the bound for structuredIntros
+              -- That amount of underscores are provided as terms to structuredIntros
+              let newGoal ← getMainGoal
+              let s ← goalsToStateDiff goal newGoal
+              match (s.newDecls, s.changedDecls, s.removedDecls) with
+              | (newDecls, #[], #[]) => 
+                -- TODO there must be an easier way to create an newDecls.size array of _
+                let mut termHoles := #[]
+                for _ in newDecls do
+                  termHoles := termHoles.push (← `( _ ))
+                structuredIntros goalType termHoles
+              | _ => throwUnsupportedSyntax
+            else
+              let termIds ← ids.mapM mapBinderIdentToTerm            
+              structuredIntros goalType termIds
+
       | `(tactic|cases $target:term) 
         => structuredCasesOrInduction tacSeq goal target false
       | `(tactic|induction $target:term)
@@ -353,13 +461,34 @@ inductive Even : Nat → Prop
 | add_two : ∀ k : Nat, Even k → Even (k+2)
 | combine_two (n : Nat) (hn : Even n) : ∀ m : Nat, Even m → Even (n + m)
 
-example (n : Nat) : n = n := by
+example : Even 4 := by
+  structured repeat apply Even.add_two _ _
+
+
+example : Even 4 := by
   structured 
-    cases n
-    try apply Even.zero
-  repeat sorry
+    have _ : Even 0 := Even.zero
 
-example : α ∧ β → β := by
-  structured intro ⟨_, _⟩ 
+  structured 
+    have x := Even.zero
 
--- TODO: Wrap defaultCases in a show .. by .. block ?
+  structured
+    have := Even.zero
+  let _ : Even 0 := Even.zero
+
+example : α₁ → α₂ ∧ α₃ → α₄ ∧ α₅ → α₆ ∧ α₇ → α₁ := by
+  structured
+    intros
+  -- intro (ha1 : α₁) (h : α₂ ∧ α₃) (h_1 : α₄ ∧ α₅) 
+  
+
+example (n m : Nat) : Even n ∧ Even m → Even 0 → Even 2 → Even (n + m) := by 
+  -- intro
+  -- intro _ 
+  -- intro hnm
+  -- intros _
+  -- intro hnm _
+  -- intros
+  -- intros hm _
+  -- structured intro ⟨hn, _⟩ _ _
+  structured intro (⟨hn, _⟩ : Even n ∧ Even m)(h : Even 0)(h_1 : Even 2)
